theories/typing/soundness.v
@@ -1,0 +1,78 @@
+From iris.algebra Require Import frac.
+From iris.base_logic Require Import big_op.
+From iris.base_logic.lib Require Import na_invariants.
+From iris.proofmode Require Import tactics.
+From lrust.lang Require Import races adequacy proofmode notation.
+From lrust.lifetime Require Import lifetime frac_borrow.
+From lrust.typing Require Import typing.
+
+Set Default Proof Using "Type".
+
+Class typePreG Σ := PreTypeG {
+  type_heapG :> heapPreG Σ;
+  type_lftG :> lftPreG Σ;
+  type_preG_na_invG :> na_invG Σ;
+  type_frac_borrowG :> frac_borG Σ
+}.
+
+Definition typeΣ : gFunctors :=
+  #[heapΣ; lftΣ; na_invΣ; GFunctor (constRF fracR)].
+Instance subG_typePreG {Σ} : subG typeΣ Σ → typePreG Σ.
+Proof.
+  split.
+  - apply subG_heapPreG. solve_inG.
+  - apply subG_lftPreG. solve_inG.
+  - solve_inG.
+  - solve_inG.
+Qed.
+
+Section type_soundness.
+  Definition exit_cont : val := λ: [<>], #().
+
+  Definition main_type `{typeG Σ} :=
+    fn (λ _, []) (λ _, [# ]) (λ _:(), box unit).
+
+  Theorem type_soundness `{typePreG Σ} (main : val) σ t :
+    (∀ `{typeG Σ}, typed_instruction_ty [] [] [] main main_type) →
+    rtc step ([main [exit_cont]%E], ∅) (t, σ) →
+    nonracing_threadpool t σ ∧
+    (∀ e, e ∈ t → is_Some (to_val e) ∨ reducible e σ).
+  Proof.
+    intros Hmain Hrtc.
+    cut (adequate (main [exit_cont]%E) ∅ (λ _, True)).
+    { split. by eapply adequate_nonracing.
+      intros. by eapply (adequate_safe (main [exit_cont]%E)). }
+    apply: heap_adequacy=>?.
+    iIntros "!# #HEAP". iMod lft_init as (?) "#LFT". done.
+    iMod na_alloc as (tid) "Htl". set (Htype := TypeG _ _ _ _ _).
+    wp_bind (of_val main). iApply (wp_wand with "[Htl]").
+    iApply (Hmain _ $! tid 1%Qp with "* HEAP LFT Htl [] [] []").
+    { by rewrite /elctx_interp big_sepL_nil. }
+    { by rewrite /llctx_interp big_sepL_nil. }
+    { by rewrite tctx_interp_nil. }
+    clear Hrtc Hmain main. iIntros (main) "(Htl & _ & _ & Hmain)".
+    rewrite tctx_interp_singleton. iDestruct "Hmain" as (?) "[EQ Hmain]".
+    rewrite eval_path_of_val. iDestruct "EQ" as %[= <-].
+    iDestruct "Hmain" as (f k x e ?) "(EQ & % & Hmain)". iDestruct "EQ" as %[= ->].
+    destruct x; try done.
+    iApply (wp_rec _ _ _ _ _ _ [exit_cont]%E); [done| |by simpl_subst|iNext].
+    { repeat econstructor. apply to_of_val. }
+    iApply ("Hmain" $! () exit_cont [#] tid 1%Qp with "HEAP LFT Htl [] [] []");
+      last by rewrite tctx_interp_nil.
+    { by rewrite /elctx_interp big_sepL_nil. }
+    { by rewrite /llctx_interp big_sepL_nil. }
+    iIntros "_". rewrite cctx_interp_singleton. simpl. iIntros (args) "_ _".
+    inv_vec args. iIntros (x) "_". by wp_seq.
+  Qed.
+End type_soundness.
+
+(* Soundness theorem when no other CMRA is needed. *)
+
+Theorem type_soundness_closed (main : val) σ t :
+  (∀ `{typeG typeΣ}, typed_instruction_ty [] [] [] main main_type) →
+  rtc step ([main [exit_cont]%E], ∅) (t, σ) →
+  nonracing_threadpool t σ ∧
+  (∀ e, e ∈ t → is_Some (to_val e) ∨ reducible e σ).
+Proof.
+  intros. eapply @type_soundness; try done. apply _.
+Qed.
