theories/typing/type_context.v
@@ -1,6 +1,5 @@
 From iris.proofmode Require Import tactics.
 From iris.base_logic Require Import big_op.
-From lrust.lang Require Import notation.
 From lrust.typing Require Import type lft_contexts.
 Set Default Proof Using "Type".
 
